src/Iris/Examples/IRun.lean
@@ -37,6 +37,53 @@ theorem irun_apply.{u} {PROP : Type u} [BI PROP] {P Q Q' : PROP}
   (h2 : P ⊢ Q')
  : P ⊢ Q := h2.trans h1
 
+def irunSearch (config : IRunConfig) (goal : MVarId) (tree : DiscrTree IRunEntry) : TacticM (Bool × List MVarId × List MVarId) := do
+  goal.withContext do
+    let mut g ← instantiateMVars <| ← goal.getType
+    let some { u, prop, bi, e, hyps, goal:=G } := parseIrisGoal? g | throwError "not in proof mode"
+    if config.debug then logInfo m!"Goal: {G}"
+    -- logInfo m!"IN LOOP: {G}"
+    let G ← instantiateExprMVars G
+    if G.isMVar then throwError "irun failed: goal has free metavars"
+    let tacs ← tree.getMatch G
+    let tacs := tacs.insertionSort λ a b => a.prio < b.prio
+    for tac in tacs do
+      if config.debug then logInfo m!"trying {tac.name}"
+      match tac.tac with
+      | .inl decl =>
+        let info ← getConstInfo decl
+        -- TODO: create new mvar level to prevent instantiating mvars in the goal, see https://leanprover.zulipchat.com/#narrow/channel/270676-lean4/topic/Difference.20between.20DiscrTree.2EgetMatch.20and.20DiscrTree.2EgetUnify/near/513194806 ?
+        let pf := mkConst decl (← mkFreshLevelMVarsFor info)
+        let (args, _, targetTy) ← forallMetaTelescopeReducing (← inferType pf)
+        let .some (Gnew, Gdecl) := (unpackEntails targetTy) | throwError "theorem is not entails, this should not happen"
+        let .true ← isDefEq G Gdecl | continue
+
+        let mut do_cont := false
+        for mvar in args do
+          let mvarId := mvar.mvarId!
+          if ! (← mvarId.isAssigned) && ! (← mvarId.isDelayedAssigned) then
+            try
+              let [] ← evalTacticAtRaw (← `(tactic|irunsolve)) mvarId | throwError "solver failed"
+            catch e =>
+              if config.debug then
+                logInfo m!"[irun] error '{e.toMessageData}' when solving uninstantiated argument `{← instantiateMVars <| ← mvarId.getType}` of lemma {tac.name}"
+              do_cont := true
+              break
+        if do_cont then continue
+
+        if config.debug then logInfo m!"successfully applied {tac.name}"
+        let m ← mkFreshExprSyntheticOpaqueMVar <|
+          IrisGoal.toExpr { prop, bi, hyps := hyps, goal := Gnew }
+        let pf := mkApp7 (.const ``irun_apply [u]) prop bi e G Gnew (mkAppN pf args) m
+        goal.assign pf
+        return (true, [m.mvarId!], [])
+      | .inr tac =>
+        let .some (goals_new, shelved_new) ← tac.tac.run goal config | continue
+        if config.debug then logInfo m!"successfully applied {tac.name}"
+        return (true, goals_new, shelved_new)
+    return (false, [goal], [])
+
+
 --def profileitM (_ : Type) (_ : String) (_ : Options) (act : TacticM α) : TacticM α := act
 partial def irunCore (config : IRunConfig) (nsteps : Option Nat) : TacticM Unit := do profileitM Exception "irun" (← getOptions) do
   -- TODO: keep track of [IrisGoal]s instead of just MVars such that tactics can avoid reparsing
@@ -47,6 +94,7 @@ partial def irunCore (config : IRunConfig) (nsteps : Option Nat) : TacticM Unit 
   --   logInfo m!"goals: {goals}"
   --   logInfo m!"shelved: {shelved}"
   let mut n := 0
+  let tree := irunExt.getState (← getEnv)
   repeat
     if nsteps == some n then
       break
@@ -99,55 +147,13 @@ partial def irunCore (config : IRunConfig) (nsteps : Option Nat) : TacticM Unit 
       goal := ← goal.replaceTargetDefEq g_new
 
     -- find a tactic or lemma to apply to the goal
-    let (progress, goals'', shelved') ← goal.withContext do
-      let mut g ← instantiateMVars <| ← goal.getType
-      let some { u, prop, bi, e, hyps, goal:=G } := parseIrisGoal? g | throwError "not in proof mode"
-      if config.debug then logInfo m!"Goal: {G}"
-      -- logInfo m!"IN LOOP: {G}"
-      let tree := irunExt.getState (← getEnv)
-      let G ← instantiateExprMVars G
-      if G.isMVar then throwError "irun failed: goal has free metavars"
-      let tacs ← tree.getMatch G
-      let tacs := tacs.insertionSort λ a b => a.prio < b.prio
-      for tac in tacs do
-        if config.debug then logInfo m!"trying {tac.name}"
-        match tac.tac with
-        | .inl decl =>
-          let info ← getConstInfo decl
-          -- TODO: create new mvar level to prevent instantiating mvars in the goal, see https://leanprover.zulipchat.com/#narrow/channel/270676-lean4/topic/Difference.20between.20DiscrTree.2EgetMatch.20and.20DiscrTree.2EgetUnify/near/513194806 ?
-          let pf := mkConst decl (← mkFreshLevelMVarsFor info)
-          let (args, _, targetTy) ← forallMetaTelescopeReducing (← inferType pf)
-          let .some (Gnew, Gdecl) := (unpackEntails targetTy) | throwError "theorem is not entails, this should not happen"
-          let .true ← isDefEq G Gdecl | continue
-
-          let mut do_cont := false
-          for mvar in args do
-            let mvarId := mvar.mvarId!
-            if ! (← mvarId.isAssigned) && ! (← mvarId.isDelayedAssigned) then
-              try
-                let [] ← evalTacticAtRaw (← `(tactic|irunsolve)) mvarId | throwError "solver failed"
-              catch e =>
-                if config.debug then
-                  logInfo m!"[irun] error '{e.toMessageData}' when solving uninstantiated argument `{← instantiateMVars <| ← mvarId.getType}` of lemma {tac.name}"
-                do_cont := true
-                break
-          if do_cont then continue
-
-          let m ← mkFreshExprSyntheticOpaqueMVar <|
-            IrisGoal.toExpr { prop, bi, hyps := hyps, goal := Gnew }
-          let pf := mkApp7 (.const ``irun_apply [u]) prop bi e G Gnew (mkAppN pf args) m
-          goal.assign pf
-          return (true, m.mvarId!::goals', shelved)
-        | .inr tac =>
-          let .some (goals_new, shelved_new) ← tac.tac.run goal config | continue
-          return (true, goals_new++goals', shelved++shelved_new)
-      return (false, goal::goals', shelved)
+    let (progress, goals_new, shelved_new) ← irunSearch config goal tree
     if !progress && !progress_match then
       if config.debug then logInfo m!"no progress, exiting"
       break
     n := n+1
-    goals := goals''
-    shelved := shelved'
+    goals := goals_new ++ goals'
+    shelved := shelved ++ shelved_new
 
   if !(nsteps == .none || nsteps == .some n) then
     logInfo s!"Did {n} steps"
